Prove stronger non-surjectivity result for `eval`

meta-theory/pure_eval_surjScript.sml
@@ -2,11 +2,11 @@
   Prove that there exists values that cannot be computed by any
   PureCake program, or in other words, that eval is surjective.
 *)
-open HolKernel Parse boolLib bossLib term_tactic;
-open arithmeticTheory listTheory stringTheory alistTheory
-     optionTheory pairTheory ltreeTheory llistTheory bagTheory pure_evalTheory
-     pred_setTheory cardinalTheory BasicProvers rich_listTheory combinTheory
-     pure_expTheory pure_valueTheory pure_exp_lemmasTheory;
+open HolKernel Parse boolLib bossLib term_tactic BasicProvers dep_rewrite;
+open arithmeticTheory listTheory stringTheory alistTheory optionTheory
+     pairTheory ltreeTheory llistTheory bagTheory cardinalTheory
+     pred_setTheory rich_listTheory combinTheory finite_mapTheory
+open pure_evalTheory pure_expTheory pure_valueTheory pure_exp_lemmasTheory;
 
 val _ = new_theory "pure_eval_surj";
 
@@ -252,10 +252,9 @@ QED
 Theorem v_lookup_gen_v:
   ∀path f.
     (∀path a len. f path = (a,len) ∧ (∀b. a ≠ Constructor' b) ⇒ len = 0) ∧
-    (∀y. y ≼ path ∧ y≠path ⇒
-       ∃b n. f y = (Constructor' b, n) ∧ EL (LENGTH y) path < n
-    ) ⇒
-    v_lookup path (gen_v f) = f path
+    (∀y. y ≼ path ∧ y ≠ path ⇒
+       ∃b n. f y = (Constructor' b, n) ∧ EL (LENGTH y) path < n)
+    ⇒ v_lookup path (gen_v f) = f path
 Proof
   Induct >> rpt strip_tac >-
     (rw[v_lookup,Once gen_v] >>
@@ -265,6 +264,7 @@ Proof
   first_assum(qspec_then ‘[]’ mp_tac) >>
   impl_tac >- simp[] >>
   strip_tac >>
+  fs[] >>
   simp[oEL_def] >>
   gvs[oEL_THM] >>
   last_x_assum(qspec_then ‘(λpath. f (h::path))’ mp_tac) >>
@@ -274,6 +274,32 @@ Proof
   first_x_assum(qspec_then ‘h::y’ mp_tac) >>
   reverse impl_tac >- simp[] >>
   simp[]
+QED
+
+Theorem v_lookup_gen_v_alt:
+  ∀path f.
+    v_lookup path (gen_v f) =
+      if (∀y. y ≼ path ∧ y ≠ path ⇒
+            ∃b n. f y = (Constructor' b, n) ∧ EL (LENGTH y) path < n) then
+        (case f path of
+            (Constructor' c, n) => (Constructor' c, n)
+          | (pre, n)            => (pre, 0))
+      else (Diverge', 0)
+Proof
+  Induct >> rpt strip_tac
+  >- (rw[v_lookup, Once gen_v] >> TOP_CASE_TAC >> gvs[AllCaseEqs()]) >>
+  reverse (rw[v_lookup, Once gen_v]) >> gvs[oEL_THM]
+  >- (
+    CASE_TAC >> CASE_TAC >> CASE_TAC >> gvs[] >>
+    IF_CASES_TAC >> gvs[] >>
+    Cases_on `y` >> gvs[] >>
+    first_x_assum (qspec_then `t` assume_tac) >> gvs[]
+    ) >>
+  first_assum(qspec_then `[]` mp_tac) >>
+  impl_tac >- simp[] >>
+  strip_tac >> fs[] >>
+  IF_CASES_TAC >> gvs[] >>
+  first_x_assum (qspec_then `h::path'` assume_tac) >> gvs[]
 QED
 
 Theorem IS_PREFIX_NOT_EQ:
@@ -356,6 +382,365 @@ Proof
   spose_not_then strip_assume_tac >>
   ‘𝕌(:v) ≼ 𝕌(:exp)’ by(metis_tac[cardleq_SURJ]) >>
   metis_tac[v_uncountable,CANTOR_THM_UNIV,cardleq_TRANS,exp_countable,COUNTABLE_ALT_cardleq]
+QED
+
+(******************************************************************************)
+
+Definition cons_names_def:
+  (cons_names (Var v) = {}) ∧
+  (cons_names (Prim op es) =
+    let cons_es = BIGUNION (set (MAP (λe. cons_names e) es)) in
+    case op of Cons c => c INSERT cons_es | _ => cons_es) ∧
+  (cons_names (App e1 e2) = cons_names e1 ∪ cons_names e2) ∧
+  (cons_names (Lam x body) = cons_names body) ∧
+  (cons_names (Letrec fs e) =
+    cons_names e ∪ BIGUNION (set (MAP (λ(f,e). cons_names e) fs)))
+Termination
+  WF_REL_TAC ‘measure exp_size’ >> fs[] >>
+  conj_tac >> TRY (Induct_on `fs`) >> TRY (Induct_on `es`) >> rw[] >>
+  gvs[fetch "pure_exp" "exp_size_def"] >> res_tac >>
+  pop_assum (assume_tac o SPEC_ALL) >> fs[]
+End
+
+Theorem cons_names_FINITE:
+  ∀e ns. cons_names e = ns ⇒ FINITE ns
+Proof
+  recInduct cons_names_ind >> reverse (rw[cons_names_def])
+  >- (gvs[MEM_MAP] >> PairCases_on `y` >> gvs[] >> res_tac) >>
+  TOP_CASE_TAC >> gvs[MEM_MAP, PULL_EXISTS]
+QED
+
+Theorem cons_names_subst:
+  ∀ f e n.
+    n ∈ cons_names (subst f e)
+  ⇒ n ∈ cons_names e ∨ (∃k e'. FLOOKUP f k = SOME e' ∧ n ∈ cons_names e')
+Proof
+  recInduct subst_ind >> rw[cons_names_def, subst_def]
+  >- (
+    FULL_CASE_TAC >> gvs[cons_names_def] >>
+    goal_assum drule >> simp[]
+    )
+  >- (
+    gvs[MAP_MAP_o, combinTheory.o_DEF] >>
+    Cases_on `∃c. op = Cons c` >> gvs[]
+    >- (
+      gvs[MEM_MAP, PULL_EXISTS, PULL_FORALL] >>
+      first_x_assum drule_all >> metis_tac[]
+      ) >>
+    `n ∈ BIGUNION (set (MAP (λa. cons_names (subst m a)) xs))` by (
+      Cases_on `op` >> gvs[MEM_MAP, PULL_EXISTS] >>
+      goal_assum drule >> simp[]) >>
+    last_x_assum assume_tac >> last_x_assum kall_tac >>
+    qsuff_tac `
+      n ∈ BIGUNION (set (MAP (λe. cons_names e) xs)) ∨
+      ∃k e'. FLOOKUP m k = SOME e' ∧ n ∈ cons_names e'`
+    >- (CASE_TAC >> gvs[]) >>
+    gvs[MEM_MAP, PULL_EXISTS, PULL_FORALL] >>
+    first_x_assum drule_all >> metis_tac[]
+    )
+  >- (first_x_assum drule >> strip_tac >> simp[] >> metis_tac[])
+  >- (first_x_assum drule >> strip_tac >> simp[] >> metis_tac[])
+  >- (
+    first_x_assum drule >> strip_tac >> simp[] >>
+    gvs[DOMSUB_FLOOKUP_THM] >> metis_tac[]
+    )
+  >- (
+    first_x_assum drule >> strip_tac >> simp[] >>
+    gvs[FDIFF_def, FLOOKUP_DRESTRICT, MEM_MAP] >>
+    metis_tac[]
+    )
+  >- (
+    gvs[MEM_MAP, PULL_EXISTS, FDIFF_def, FLOOKUP_DRESTRICT] >>
+    rename1 `MEM foo _` >> PairCases_on `foo` >> gvs[EXISTS_PROD] >>
+    first_x_assum drule_all >> strip_tac >> metis_tac[]
+    )
+QED
+
+Theorem cons_names_bind:
+  ∀ f e n.
+    n ∈ cons_names (bind f e)
+  ⇒ n ∈ cons_names e ∨ (∃k e'. FLOOKUP f k = SOME e' ∧ n ∈ cons_names e')
+Proof
+  rw[bind_def, cons_names_def] >>
+  irule cons_names_subst >> simp[]
+QED
+
+Theorem cons_names_bind_single:
+  ∀ x e' e n.
+    n ∈ cons_names (bind x e' e)
+  ⇒ n ∈ cons_names e ∨ n ∈ cons_names e'
+Proof
+  rw[] >>
+  drule cons_names_bind >> strip_tac >> simp[] >>
+  gvs[FLOOKUP_UPDATE]
+QED
+
+Theorem cons_names_subst_funs:
+  ∀ f e n.
+    n ∈ cons_names (subst_funs f e)
+  ⇒ n ∈ cons_names e ∨ (∃e'. MEM e' (MAP SND f) ∧ n ∈ cons_names e')
+Proof
+  rw[subst_funs_def] >>
+  drule cons_names_bind >> strip_tac >> simp[] >>
+  gvs[flookup_fupdate_list] >> FULL_CASE_TAC >> gvs[] >>
+  imp_res_tac ALOOKUP_MEM >>
+  gvs[MEM_REVERSE, MEM_MAP, PULL_EXISTS] >>
+  PairCases_on `y` >> gvs[cons_names_def]
+  >- (DISJ2_TAC >> goal_assum drule >> simp[]) >>
+  gvs[MEM_MAP] >> PairCases_on `y` >> gvs[cons_names_def] >>
+  DISJ2_TAC >> qexists_tac `(y0,y1')` >> simp[]
+QED
+
+Definition cons_names_wh_def:
+  (cons_names_wh (wh_Constructor c es) =
+    c INSERT BIGUNION (set (MAP (λe. cons_names e) es))) ∧
+  (cons_names_wh (wh_Closure x body) = cons_names body) ∧
+  (cons_names_wh _ = {})
+End
+
+Theorem cons_name_wh_trivial_simps[simp]:
+  (∀a. cons_names_wh (wh_Atom a) = {}) ∧
+  (∀x body. cons_names_wh (wh_Closure x body) = cons_names body) ∧
+  (cons_names_wh wh_Error = {}) ∧
+  (cons_names_wh wh_Diverge = {})
+Proof
+  rw[cons_names_wh_def]
+QED
+
+Theorem cons_name_wh_FINITE:
+  ∀wh ns. cons_names_wh wh = ns ⇒ FINITE ns
+Proof
+  reverse Induct >> rw[cons_names_wh_def]
+  >- (metis_tac[cons_names_FINITE]) >>
+  gvs[FINITE_INSERT, MEM_MAP, PULL_EXISTS] >> rw[] >>
+  metis_tac[cons_names_FINITE]
+QED
+
+Definition cons_names_v_def:
+  cons_names_v v =
+    {c | ∃path n. v_lookup path v = (Constructor' c, n)} ∪
+    BIGUNION {cons_names e | ∃path x n. v_lookup path v = (Closure' x e, n)}
+End
+
+Theorem cons_names_v:
+  (∀a. cons_names_v (Atom a) = {}) ∧
+  (∀c vs. cons_names_v (Constructor c vs) =
+    c INSERT BIGUNION (set (MAP (λv. cons_names_v v) vs))) ∧
+  (∀x body. cons_names_v (Closure x body) = cons_names body) ∧
+  (cons_names_v Diverge = {}) ∧
+  (cons_names_v Error = {})
+Proof
+  rw[cons_names_v_def, EXTENSION, DISJ_EQ_IMP, PULL_EXISTS]
+  >- (Cases_on `path` >> gvs[v_lookup])
+  >- (Cases_on `path` >> gvs[v_lookup])
+  >- (
+    rename1 `Constructor' c'` >> eq_tac >> rw[]
+    >- (
+      gvs[MEM_MAP, PULL_EXISTS] >>
+      simp[DISJ_EQ_IMP] >> gvs[GSYM EXTENSION] >>
+      reverse (Cases_on
+        `∀path n. v_lookup path (Constructor c vs) ≠ (Constructor' c', n)`) >>
+      gvs[]
+      >- (
+        Cases_on `path` >> gvs[v_lookup, oEL_THM] >>
+        FULL_CASE_TAC >> gvs[] >>
+        qexists_tac `EL h vs` >> gvs[EL_MEM] >> rw[] >> res_tac
+        ) >>
+      rename1 `Closure' x body` >>
+      Cases_on `path` >> gvs[v_lookup, oEL_THM] >>
+      FULL_CASE_TAC >> gvs[] >>
+      qexists_tac `EL h vs` >> gvs[EL_MEM] >> rw[] >>
+      goal_assum drule >> goal_assum drule
+      )
+    >- (
+      Cases_on `c' = c` >> gvs[]
+      >- (first_x_assum (qspec_then `[]` assume_tac) >> gvs[v_lookup]) >>
+      gvs[MEM_MAP, MEM_EL]
+      >- (
+        rename1 `foo < _` >>
+        first_x_assum (qspec_then `foo::path` assume_tac) >>
+        gvs[v_lookup, oEL_THM]
+        ) >>
+      simp[GSYM EXTENSION] >> goal_assum drule >>
+      qexists_tac `n::path` >> gvs[v_lookup, oEL_THM]
+      )
+    )
+  >- (
+    rename1 `Constructor' c` >>
+    `∀path n. v_lookup path (Closure x body) ≠ (Constructor' c, n)` by (
+      Cases >> rw[v_lookup]) >>
+    simp[] >> eq_tac >> rw[]
+    >- (Cases_on `path` >> gvs[v_lookup]) >>
+    goal_assum drule >>
+    qexistsl_tac [`body`,`[]`,`x`,`0`] >> gvs[v_lookup]
+    ) >>
+  Cases_on `path` >> gvs[v_lookup]
+QED
+
+Triviality REPLICATE_11:
+  ∀n m e. REPLICATE n e = REPLICATE m e ⇒ n = m
+Proof
+  Induct >> rw[] >>
+  Cases_on `m` >> gvs[] >>
+  first_x_assum irule >> goal_assum drule
+QED
+
+Theorem cons_names_v_exists_INFINITE:
+  ∃v. INFINITE (cons_names_v v)
+Proof
+  rw[infinite_num_inj, INJ_DEF] >>
+  qexists_tac
+    `gen_v (λpath. (Constructor' (REPLICATE (LENGTH path) #"a"), 1))` >>
+  qexists_tac `λn. REPLICATE n #"a"` >> reverse (rw[])
+  >- (drule REPLICATE_11 >> simp[]) >>
+  simp[cons_names_v_def, DISJ_EQ_IMP, PULL_EXISTS] >>
+  rename1 `_ ⇒ false` >> rw[] >>
+  CCONTR_TAC >> last_x_assum mp_tac >> simp[] >>
+  qexistsl_tac [`REPLICATE x 0`,`1`] >>
+  dep_rewrite.DEP_ONCE_REWRITE_TAC [v_lookup_gen_v] >>
+  simp[] >> rw[] >>
+  dep_rewrite.DEP_ONCE_REWRITE_TAC [EL_REPLICATE] >> simp[] >>
+  drule IS_PREFIX_NOT_EQ >> gvs[]
+QED
+
+Definition cons_names_v_prefix_def[simp]:
+  (cons_names_v_prefix (Constructor' c) = {c}) ∧
+  (cons_names_v_prefix (Closure' x body) = cons_names body) ∧
+  (cons_names_v_prefix _ = {})
+End
+
+Definition add_TF_def:
+  add_TF s = s ∪ {"True";"False"}
+End
+
+Theorem cons_names_eval_wh_to:
+  ∀ k e wh n.
+    eval_wh_to k e = wh ∧
+    n ∈ cons_names_wh wh
+  ⇒ n ∈ add_TF (cons_names e)
+Proof
+  recInduct eval_wh_to_ind >> rw[eval_wh_to_def] >> gvs[cons_names_def]
+  >- simp[add_TF_def]
+  >- (
+    Cases_on `eval_wh_to k x` >> gvs[dest_wh_Closure_def] >>
+    FULL_CASE_TAC >> gvs[] >>
+    first_x_assum drule >> strip_tac >>
+    gvs[add_TF_def] >>
+    drule cons_names_bind >> simp[FLOOKUP_UPDATE] >>
+    strip_tac >> metis_tac[]
+    )
+  >- (
+    first_x_assum drule >> strip_tac >>
+    gvs[MEM_MAP, PULL_EXISTS, EXISTS_PROD, add_TF_def] >>
+    drule cons_names_subst_funs >> strip_tac >> simp[] >>
+    gvs[MEM_MAP] >> rename1 `MEM foo _` >> PairCases_on `foo` >> gvs[] >>
+    metis_tac[]
+    )
+  >- (
+    Cases_on `∃c. p = Cons c` >> gvs[cons_names_wh_def, add_TF_def]
+    >- metis_tac[] >>
+    qsuff_tac
+      `n ∈ BIGUNION (set (MAP (λe. cons_names e) xs)) ∨ n = "True" ∨ n = "False"`
+    >- (CASE_TAC >> gvs[]) >>
+    Cases_on `p` >> gvs[MEM_MAP, PULL_EXISTS]
+    >- (
+      Cases_on `xs` >> gvs[] >> Cases_on `t` >> gvs[] >>
+      EVERY_CASE_TAC >> gvs[cons_names_wh_def]
+      )
+    >- (
+      Cases_on `xs` >> gvs[] >> Cases_on `t` >> gvs[] >>
+      EVERY_CASE_TAC >> gvs[cons_names_wh_def] >>
+      first_x_assum drule >> strip_tac >> simp[] >>
+      first_x_assum irule >> gvs[MEM_MAP, PULL_EXISTS, MEM_EL] >>
+      metis_tac[]
+      ) >>
+    EVERY_CASE_TAC >> gvs[]
+    )
+  >- (
+    Cases_on `∃c. p = Cons c` >> gvs[cons_names_wh_def, add_TF_def]
+    >- metis_tac[] >>
+    qsuff_tac
+      `n ∈ BIGUNION (set (MAP (λe. cons_names e) xs)) ∨ n = "True" ∨ n = "False"`
+    >- (CASE_TAC >> gvs[]) >>
+    Cases_on `p` >> gvs[MEM_MAP, PULL_EXISTS]
+    >- (
+      Cases_on `xs` >> gvs[] >> Cases_on `t` >> gvs[] >>
+      Cases_on `t'` >> gvs[] >> Cases_on `t` >> gvs[] >>
+      EVERY_CASE_TAC >> gvs[cons_names_wh_def, PULL_FORALL] >>
+      first_x_assum (drule_at Any) >> strip_tac >> gvs[] >>
+      metis_tac[]
+      ) >>
+    EVERY_CASE_TAC >> gvs[]
+    )
+QED
+
+Theorem cons_names_eval_wh:
+  ∀e wh n.
+    eval_wh e = wh ∧
+    n ∈ cons_names_wh wh
+  ⇒ n ∈ add_TF (cons_names e)
+Proof
+  rw[eval_wh_def] >> FULL_CASE_TAC >> gvs[] >>
+  last_x_assum mp_tac >> DEEP_INTRO_TAC some_intro >> rw[] >>
+  irule cons_names_eval_wh_to >> irule_at Any EQ_REFL >>
+  goal_assum drule
+QED
+
+Theorem cons_names_follow_path_eval_wh:
+  ∀path e pre n nm.
+    follow_path eval_wh e path = (pre, n) ∧
+    nm ∈ cons_names_v_prefix pre
+  ⇒ nm ∈ add_TF (cons_names e)
+Proof
+  Induct >> rw[follow_path_def]
+  >- (
+    EVERY_CASE_TAC >> gvs[] >>
+    irule cons_names_eval_wh >> simp[cons_names_wh_def]
+    ) >>
+  EVERY_CASE_TAC >> gvs[oEL_THM] >>
+  first_x_assum drule_all >>
+  gvs[add_TF_def] >> strip_tac >> simp[] >>
+  drule cons_names_eval_wh >>
+  simp[cons_names_wh_def, MEM_MAP, PULL_EXISTS, add_TF_def] >>
+  disch_then irule >> DISJ2_TAC >>
+  goal_assum drule >> gvs[EL_MEM]
+QED
+
+Theorem cons_names_gen_v_follow_path_eval_wh:
+  ∀e v n.
+    gen_v (follow_path eval_wh e) = v ∧
+    n ∈ cons_names_v v
+  ⇒ n ∈ add_TF (cons_names e)
+Proof
+  gvs[cons_names_v_def, PULL_EXISTS, PULL_FORALL, v_lookup_gen_v_alt] >>
+  rw[] >> pop_assum mp_tac >> IF_CASES_TAC >> gvs[] >>
+  EVERY_CASE_TAC >> gvs[] >> rw[] >>
+  irule cons_names_follow_path_eval_wh >>
+  goal_assum drule >> simp[]
+QED
+
+Theorem cons_names_eval:
+  ∀e v n.
+    eval e = v ∧
+    n ∈ cons_names_v v
+  ⇒ n ∈ add_TF (cons_names e)
+Proof
+  rw[eval_def, v_unfold_def] >>
+  irule cons_names_gen_v_follow_path_eval_wh >>
+  irule_at Any EQ_REFL >> simp[]
+QED
+
+Theorem eval_not_surj_strong:
+  ¬SURJ eval 𝕌(:exp) 𝕌(:v)
+Proof
+  rw[SURJ_DEF] >>
+  assume_tac cons_names_v_exists_INFINITE >> fs[] >>
+  qexists_tac `v` >> rw[] >>
+  CCONTR_TAC >> fs[] >>
+  drule cons_names_eval >> simp[] >>
+  `FINITE (add_TF (cons_names y))` by (
+    fs[add_TF_def] >> metis_tac[cons_names_FINITE]) >>
+  irule IN_INFINITE_NOT_FINITE >> simp[]
 QED
 
 val _ = export_theory();
